disk-betree/ImplModelCache.i.dfy
@@ -75,31 +75,79 @@ module ImplModelCache {
     getFreeRef2Iterate(s, avoid, 1)
   }
 
+  // Conditions that will hold intermediately between writes and allocs
+  predicate WriteAllocConditions(k: Constants, s: Variables)
+  {
+    && s.Ready?
+    && MutableMapModel.Inv(s.ephemeralIndirectionTable)
+    && (forall loc |
+        loc in IIndirectionTable(s.ephemeralIndirectionTable).locs.Values :: 
+          BC.ValidLocationForNode(loc))
+    && ConsistentBitmap(s.ephemeralIndirectionTable, s.frozenIndirectionTable,
+        s.persistentIndirectionTable, s.outstandingBlockWrites, s.blockAllocator)
+    && ImplModelBlockAllocator.Inv(s.blockAllocator)
+    && BC.AllLocationsForDifferentRefsDontOverlap(
+        IIndirectionTable(s.ephemeralIndirectionTable))
+  }
+
+  lemma lemmaIndirectionTableLocIndexValid(k: Constants, s: Variables, ref: BT.G.Reference)
+  requires WriteAllocConditions(k, s)
+  ensures ref in s.ephemeralIndirectionTable.contents && s.ephemeralIndirectionTable.contents[ref].0.Some? ==>
+    (
+      && 0 <= s.ephemeralIndirectionTable.contents[ref].0.value.addr as int / BlockSize() < NumBlocks()
+      && (s.ephemeralIndirectionTable.contents[ref].0.value.addr as int / BlockSize()) * BlockSize() == s.ephemeralIndirectionTable.contents[ref].0.value.addr as int
+    )
+  {
+    if ref in s.ephemeralIndirectionTable.contents && s.ephemeralIndirectionTable.contents[ref].0.Some? {
+      reveal_ConsistentBitmap();
+      var loc := s.ephemeralIndirectionTable.contents[ref].0.value;
+      var i := loc.addr as int / BlockSize();
+      assert IIndirectionTable(s.ephemeralIndirectionTable).locs[ref] == loc;
+      assert loc in IIndirectionTable(s.ephemeralIndirectionTable).locs.Values;
+      assert BC.ValidLocationForNode(loc);
+      LBAType.reveal_ValidAddr();
+      assert i * BlockSize() == loc.addr as int;
+      assert IsLocAllocBitmap(s.blockAllocator.ephemeral, i);
+    }
+  }
+
   // Bookkeeping only - we update the cache with the Node separately.
   // This turns out to be easier to do.
 
   function {:opaque} writeBookkeeping(k: Constants, s: Variables, ref: BT.G.Reference, children: Option<seq<BT.G.Reference>>)
   : (s': Variables)
-  requires s.Ready?
-  requires MutableMapModel.Inv(s.ephemeralIndirectionTable)
+  requires WriteAllocConditions(k, s)
   ensures s'.Ready?
   ensures s'.cache == s.cache
-  ensures MutableMapModel.Inv(s'.ephemeralIndirectionTable)
+  ensures WriteAllocConditions(k, s')
   {
+    lemmaIndirectionTableLocIndexValid(k, s, ref);
     assume s.ephemeralIndirectionTable.count as nat < 0x10000000000000000 / 8;
-    var eph := MutableMapModel.Insert(s.ephemeralIndirectionTable, ref,
+    var (eph, oldEntry) := MutableMapModel.InsertAndGetOld(s.ephemeralIndirectionTable, ref,
         (None, if children.Some? then children.value else []));
-    s.(ephemeralIndirectionTable := eph)
-        .(lru := LruModel.Use(s.lru, ref))
+    var blockAllocator' := if oldEntry.Some? && oldEntry.value.0.Some?
+      then ImplModelBlockAllocator.MarkFreeEphemeral(s.blockAllocator, oldEntry.value.0.value.addr as int / BlockSize())
+      else s.blockAllocator;
+    var s' := s.(ephemeralIndirectionTable := eph)
+     .(lru := LruModel.Use(s.lru, ref))
+     .(blockAllocator := blockAllocator');
+
+    freeIndirectionTableLocCorrect(k, s, s', ref,
+      if oldEntry.Some? && oldEntry.value.0.Some?
+      then Some(oldEntry.value.0.value.addr as int / BlockSize())
+      else None);
+    reveal_ConsistentBitmap();
+
+    s'
   }
 
   function {:opaque} allocBookkeeping(k: Constants, s: Variables, children: Option<seq<BT.G.Reference>>)
   : (p: (Variables, Option<Reference>))
-  requires s.Ready?
-  requires MutableMapModel.Inv(s.ephemeralIndirectionTable)
+  requires WriteAllocConditions(k, s)
+
   ensures var (s', id) := p;
     && s'.Ready?
-    && MutableMapModel.Inv(s'.ephemeralIndirectionTable)
+    && WriteAllocConditions(k, s')
   {
     var ref := getFreeRef(s);
     if ref.Some? then (
@@ -116,23 +164,34 @@ module ImplModelCache {
 
   function writeWithNode(k: Constants, s: Variables, ref: BT.G.Reference, node: Node)
   : (s': Variables)
-  requires s.Ready?
-  requires MutableMapModel.Inv(s.ephemeralIndirectionTable)
-  ensures s'.Ready?
+  requires WriteAllocConditions(k, s)
+  ensures WriteAllocConditions(k, s')
   {
+    lemmaIndirectionTableLocIndexValid(k, s, ref);
     assume s.ephemeralIndirectionTable.count as nat < 0x10000000000000000 / 8;
-    var eph := MutableMapModel.Insert(s.ephemeralIndirectionTable, ref,
+    var (eph, oldEntry) := MutableMapModel.InsertAndGetOld(s.ephemeralIndirectionTable, ref,
         (None, if node.children.Some? then node.children.value else []));
-    s.(ephemeralIndirectionTable := eph).(cache := s.cache[ref := node])
+    var blockAllocator' := if oldEntry.Some? && oldEntry.value.0.Some?
+      then ImplModelBlockAllocator.MarkFreeEphemeral(s.blockAllocator, oldEntry.value.0.value.addr as int / BlockSize())
+      else s.blockAllocator;
+    var s' := s.(ephemeralIndirectionTable := eph).(cache := s.cache[ref := node])
         .(lru := LruModel.Use(s.lru, ref))
+        .(blockAllocator := blockAllocator');
+
+    freeIndirectionTableLocCorrect(k, s, s', ref,
+      if oldEntry.Some? && oldEntry.value.0.Some?
+      then Some(oldEntry.value.0.value.addr as int / BlockSize())
+      else None);
+    reveal_ConsistentBitmap();
+
+    s'
   }
 
   function allocWithNode(k: Constants, s: Variables, node: Node)
   : (p: (Variables, Option<Reference>))
-  requires s.Ready?
-  requires MutableMapModel.Inv(s.ephemeralIndirectionTable)
+  requires WriteAllocConditions(k, s)
   ensures var (s', id) := p;
-    s'.Ready?
+      WriteAllocConditions(k, s')
   {
     var ref := getFreeRef(s);
     if ref.Some? then (
@@ -142,27 +201,195 @@ module ImplModelCache {
     )
   }
 
+  lemma freeIndirectionTableLocCorrect(
+      k: Constants, s: Variables, s': Variables, ref: BT.G.Reference, j: Option<int>)
+  requires WriteAllocConditions(k, s)
+  requires s'.Ready?
+  requires forall r | r != ref ::
+      MapsAgreeOnKey(
+          IIndirectionTable(s.ephemeralIndirectionTable).locs,
+          IIndirectionTable(s'.ephemeralIndirectionTable).locs,
+          r)
+  requires ref !in IIndirectionTable(s'.ephemeralIndirectionTable).locs
+  requires j.Some? ==> 0 <= j.value < NumBlocks()
+  requires j.Some? ==> ref in IIndirectionTable(s.ephemeralIndirectionTable).locs
+  requires j.Some? ==> IIndirectionTable(s.ephemeralIndirectionTable).locs[ref].addr as int == j.value * BlockSize()
+  requires j.Some? ==> s'.blockAllocator == ImplModelBlockAllocator.MarkFreeEphemeral(s.blockAllocator, j.value)
+  requires j.None? ==> s'.blockAllocator == s.blockAllocator
+  requires j.None? ==> ref !in IIndirectionTable(s.ephemeralIndirectionTable).locs
+  ensures (forall i: int :: IsLocAllocIndirectionTable(s'.ephemeralIndirectionTable, i)
+      <==> IsLocAllocBitmap(s'.blockAllocator.ephemeral, i))
+  ensures ImplModelBlockAllocator.Inv(s'.blockAllocator)
+  ensures BC.AllLocationsForDifferentRefsDontOverlap(
+        IIndirectionTable(s'.ephemeralIndirectionTable))
+  ensures (forall loc |
+        loc in IIndirectionTable(s'.ephemeralIndirectionTable).locs.Values :: 
+          BC.ValidLocationForNode(loc))
+  {
+    reveal_ConsistentBitmap();
+    Bitmap.reveal_IsSet();
+    Bitmap.reveal_BitUnset();
+    lemmaIndirectionTableLocIndexValid(k, s, ref);
+
+    forall r1, r2 | r1 in IIndirectionTable(s'.ephemeralIndirectionTable).locs && r2 in IIndirectionTable(s'.ephemeralIndirectionTable).locs
+    ensures BC.LocationsForDifferentRefsDontOverlap(IIndirectionTable(s'.ephemeralIndirectionTable), r1, r2)
+    {
+      assert MapsAgreeOnKey( IIndirectionTable(s.ephemeralIndirectionTable).locs, IIndirectionTable(s'.ephemeralIndirectionTable).locs, r1);
+      assert MapsAgreeOnKey( IIndirectionTable(s.ephemeralIndirectionTable).locs, IIndirectionTable(s'.ephemeralIndirectionTable).locs, r2);
+    }
+
+    forall loc | loc in IIndirectionTable(s'.ephemeralIndirectionTable).locs.Values
+    ensures BC.ValidLocationForNode(loc)
+    {
+      var r :| r in IIndirectionTable(s'.ephemeralIndirectionTable).locs && IIndirectionTable(s'.ephemeralIndirectionTable).locs[r] == loc;
+      assert MapsAgreeOnKey(IIndirectionTable(s.ephemeralIndirectionTable).locs, IIndirectionTable(s'.ephemeralIndirectionTable).locs, r);
+    }
+
+    if j.Some? {
+      assert BC.ValidLocationForNode(IIndirectionTable(s.ephemeralIndirectionTable).locs[ref]);
+    }
+
+    forall i: int
+    | IsLocAllocIndirectionTable(s'.ephemeralIndirectionTable, i)
+    ensures IsLocAllocBitmap(s'.blockAllocator.ephemeral, i)
+    {
+      if j.Some? && i == j.value {
+        if i == 0 {
+          assert false;
+        } else {
+          var r :| r in s'.ephemeralIndirectionTable.contents && s'.ephemeralIndirectionTable.contents[r].0.Some? &&
+              s'.ephemeralIndirectionTable.contents[r].0.value.addr as int == i * BlockSize() as int;
+          assert MapsAgreeOnKey(
+            IIndirectionTable(s.ephemeralIndirectionTable).locs,
+            IIndirectionTable(s'.ephemeralIndirectionTable).locs, r);
+
+          assert BC.LocationsForDifferentRefsDontOverlap(IIndirectionTable(s.ephemeralIndirectionTable), ref, r);
+
+          assert ref !in IIndirectionTable(s'.ephemeralIndirectionTable).locs;
+          assert r in IIndirectionTable(s'.ephemeralIndirectionTable).locs;
+          assert IIndirectionTable(s.ephemeralIndirectionTable).locs[r]
+              == IIndirectionTable(s.ephemeralIndirectionTable).locs[ref];
+          assert r == ref;
+
+          assert false;
+        }
+      } else {
+        if i == 0 {
+          assert IsLocAllocIndirectionTable(s.ephemeralIndirectionTable, i);
+          assert IsLocAllocBitmap(s.blockAllocator.ephemeral, i);
+          assert IsLocAllocBitmap(s'.blockAllocator.ephemeral, i);
+        } else {
+          var r :| r in s'.ephemeralIndirectionTable.contents && s'.ephemeralIndirectionTable.contents[r].0.Some? &&
+              s'.ephemeralIndirectionTable.contents[r].0.value.addr as int == i * BlockSize() as int;
+          //assert r != ref;
+          assert MapsAgreeOnKey(
+            IIndirectionTable(s.ephemeralIndirectionTable).locs,
+            IIndirectionTable(s'.ephemeralIndirectionTable).locs, r);
+          //assert r in IIndirectionTable(s'.ephemeralIndirectionTable).locs;
+          //assert r in IIndirectionTable(s.ephemeralIndirectionTable).locs;
+          //assert r in s.ephemeralIndirectionTable.contents;
+          //assert s.ephemeralIndirectionTable.contents[r].0.Some?;
+          //assert s.ephemeralIndirectionTable.contents[r].0.value.addr as int == i * BlockSize() as int;
+          assert IsLocAllocIndirectionTable(s.ephemeralIndirectionTable, i);
+          assert IsLocAllocBitmap(s.blockAllocator.ephemeral, i);
+          assert IsLocAllocBitmap(s'.blockAllocator.ephemeral, i);
+        }
+      }
+    }
+
+    forall i: int
+    | IsLocAllocBitmap(s'.blockAllocator.ephemeral, i)
+    ensures IsLocAllocIndirectionTable(s'.ephemeralIndirectionTable, i)
+    {
+      if j.Some? && i == j.value {
+        assert IsLocAllocIndirectionTable(s'.ephemeralIndirectionTable, i);
+      } else {
+        assert IsLocAllocBitmap(s.blockAllocator.ephemeral, i);
+        assert IsLocAllocIndirectionTable(s.ephemeralIndirectionTable, i);
+        if i == 0 {
+          assert IsLocAllocIndirectionTable(s'.ephemeralIndirectionTable, i);
+        } else {
+          var r :| r in s.ephemeralIndirectionTable.contents && s.ephemeralIndirectionTable.contents[r].0.Some? &&
+            s.ephemeralIndirectionTable.contents[r].0.value.addr as int == i * BlockSize() as int;
+          assert MapsAgreeOnKey(
+            IIndirectionTable(s.ephemeralIndirectionTable).locs,
+            IIndirectionTable(s'.ephemeralIndirectionTable).locs, r);
+          assert r in s'.ephemeralIndirectionTable.contents && s'.ephemeralIndirectionTable.contents[r].0.Some? &&
+            s'.ephemeralIndirectionTable.contents[r].0.value.addr as int == i * BlockSize() as int;
+          assert IsLocAllocIndirectionTable(s'.ephemeralIndirectionTable, i);
+        }
+      }
+    }
+
+    if j.Some? {
+      forall i | 0 <= i < NumBlocks()
+      ensures Bitmap.IsSet(s'.blockAllocator.full, i) == (
+        || Bitmap.IsSet(s'.blockAllocator.ephemeral, i)
+        || (s'.blockAllocator.frozen.Some? && Bitmap.IsSet(s'.blockAllocator.frozen.value, i))
+        || Bitmap.IsSet(s'.blockAllocator.persistent, i)
+        || Bitmap.IsSet(s'.blockAllocator.full, i)
+      )
+      {
+        if i == j.value {
+        } else {
+          assert Bitmap.IsSet(s'.blockAllocator.full, i) == Bitmap.IsSet(s.blockAllocator.full, i);
+          assert Bitmap.IsSet(s'.blockAllocator.ephemeral, i) == Bitmap.IsSet(s.blockAllocator.ephemeral, i);
+          assert s'.blockAllocator.frozen.Some? ==> Bitmap.IsSet(s'.blockAllocator.frozen.value, i) == Bitmap.IsSet(s.blockAllocator.frozen.value, i);
+          assert Bitmap.IsSet(s'.blockAllocator.persistent, i) == Bitmap.IsSet(s.blockAllocator.persistent, i);
+          assert Bitmap.IsSet(s'.blockAllocator.outstanding, i) == Bitmap.IsSet(s.blockAllocator.outstanding, i);
+        }
+      }
+    } else {
+    }
+  }
+
+  lemma writeBookkeepingBitmapCorrect(k: Constants, s: Variables, ref: BT.G.Reference, children: Option<seq<BT.G.Reference>>)
+  requires WriteAllocConditions(k, s)
+  ensures var s' := writeBookkeeping(k, s, ref, children);
+    && WriteAllocConditions(k, s')
+  {
+    /*reveal_writeBookkeeping();
+    var s' := writeBookkeeping(k, s, ref, children);
+
+    lemmaIndirectionTableLocIndexValid(k, s, ref);
+    assume s.ephemeralIndirectionTable.count as nat < 0x10000000000000000 / 8;
+    var (eph, oldEntry) := MutableMapModel.InsertAndGetOld(s.ephemeralIndirectionTable, ref,
+        (None, if children.Some? then children.value else []));
+
+    var j := if oldEntry.Some? && oldEntry.value.0.Some? then
+      Some(oldEntry.value.0.value.addr as int / BlockSize())
+    else
+      None;
+    freeIndirectionTableLocCorrect(k, s, s', ref, j);
+    reveal_ConsistentBitmap();*/
+  }
+
   lemma allocCorrect(k: Constants, s: Variables, node: Node)
-  requires s.Ready?
   requires WFVars(s)
-  requires WFNode(node)
+  requires WriteAllocConditions(k, s)
   requires BC.BlockPointsToValidReferences(INode(node), IIndirectionTable(s.ephemeralIndirectionTable).graph)
   requires TotalCacheSize(s) <= MaxCacheSize() - 1
+  requires WFNode(node)
   ensures var (s', ref) := allocWithNode(k, s, node);
     && WFVars(s')
     && (ref.Some? ==> BC.Alloc(Ik(k), IVars(s), IVars(s'), ref.value, INode(node)))
     && (ref.None? ==> s' == s)
     && (ref.Some? ==> TotalCacheSize(s') == TotalCacheSize(s) + 1)
+    && WriteAllocConditions(k, s')
   {
     var ref := getFreeRef(s);
     if ref.Some? {
+      lemmaIndirectionTableLocIndexValid(k, s, ref.value);
       LruModel.LruUse(s.lru, ref.value);
+      writeBookkeepingBitmapCorrect(k, s, ref.value, node.children);
+      reveal_writeBookkeeping();
     }
   }
   
   lemma writeCorrect(k: Constants, s: Variables, ref: BT.G.Reference, node: Node)
   requires s.Ready?
   requires WFVars(s)
+  requires WriteAllocConditions(k, s)
   requires ref in IIndirectionTable(s.ephemeralIndirectionTable).graph
   requires ref in s.cache
   requires WFNode(node)
@@ -172,10 +399,15 @@ module ImplModelCache {
     && WFVars(s')
     && BC.Dirty(Ik(k), IVars(s), IVars(s'), ref, INode(node))
     && TotalCacheSize(s') == TotalCacheSize(s)
+    && WriteAllocConditions(k, s')
   {
+    lemmaIndirectionTableLocIndexValid(k, s, ref);
     WeightBucketEmpty();
 
     LruModel.LruUse(s.lru, ref);
+
+    writeBookkeepingBitmapCorrect(k, s, ref, node.children);
+    reveal_writeBookkeeping();
 
     var s' := writeWithNode(k, s, ref, node);
     assert WFVars(s');
@@ -184,6 +416,7 @@ module ImplModelCache {
   lemma writeNewRefIsAlloc(k: Constants, s: Variables, ref: BT.G.Reference, node: Node)
   requires s.Ready?
   requires WFVars(s)
+  requires WriteAllocConditions(k, s)
   requires RefAvailable(s, ref)
   requires WFNode(node)
   requires TotalCacheSize(s) <= MaxCacheSize() - 1
@@ -192,8 +425,12 @@ module ImplModelCache {
     && WFVars(s')
     && BC.Alloc(Ik(k), IVars(s), IVars(s'), ref, INode(node))
     && TotalCacheSize(s') == TotalCacheSize(s) + 1
+    && WriteAllocConditions(k, s')
   {
     LruModel.LruUse(s.lru, ref);
+
+    writeBookkeepingBitmapCorrect(k, s, ref, node.children);
+    reveal_writeBookkeeping();
   }
 
   lemma lemmaChildInGraph(k: Constants, s: Variables, ref: BT.G.Reference, childref: BT.G.Reference)
