disk-betree/ImplCache.i.dfy
@@ -81,26 +81,32 @@ module ImplCache {
   }
 
   method writeBookkeeping(k: ImplConstants, s: ImplVariables, ref: BT.G.Reference, children: Option<seq<BT.G.Reference>>)
-  requires s.ready
   requires s.W()
   requires |LruModel.I(s.lru.Queue)| <= 0x1_0000_0000
+  requires ImplModelCache.WriteAllocConditions(Ic(k), s.I())
   modifies s.lru.Repr
   modifies s.ephemeralIndirectionTable.Repr
-  ensures s.ready
+  modifies s.blockAllocator.Repr
   ensures s.W()
+  ensures s.I() == ImplModelCache.writeBookkeeping(Ic(k), old(s.I()), ref, children)
   ensures forall o | o in s.lru.Repr :: o in old(s.lru.Repr) || fresh(o)
   ensures forall o | o in s.ephemeralIndirectionTable.Repr :: o in old(s.ephemeralIndirectionTable.Repr) || fresh(o)
-  ensures s.I() == ImplModelCache.writeBookkeeping(Ic(k), old(s.I()), ref, children)
+  ensures forall o | o in s.blockAllocator.Repr :: o in old(s.blockAllocator.Repr) || fresh(o)
   ensures |LruModel.I(s.lru.Queue)| <= |LruModel.I(old(s.lru.Queue))| + 1
-  //ensures s.cache.I() == old(s.cache.I())
   {
     ImplModelCache.reveal_writeBookkeeping();
 
+    ImplModelCache.lemmaIndirectionTableLocIndexValid(Ic(k), s.I(), ref);
+
     // TODO how do we deal with this?
     assume s.ephemeralIndirectionTable.Count as nat < 0x10000000000000000 / 8;
-    s.ephemeralIndirectionTable.Insert(ref, (None, if children.Some? then children.value else []));
+    var oldEntry := s.ephemeralIndirectionTable.InsertAndGetOld(ref, (None, if children.Some? then children.value else []));
 
     s.lru.Use(ref);
+
+    if oldEntry.Some? && oldEntry.value.0.Some? {
+      s.blockAllocator.MarkFreeEphemeral(oldEntry.value.0.value.addr / BlockSizeUint64());
+    }
 
     LruModel.LruUse(old(s.lru.Queue), ref);
     assert LruModel.I(s.lru.Queue) == LruModel.I(old(s.lru.Queue)) + {ref};
@@ -111,19 +117,19 @@ module ImplCache {
 
   method allocBookkeeping(k: ImplConstants, s: ImplVariables, children: Option<seq<BT.G.Reference>>)
   returns (ref: Option<BT.G.Reference>)
-  requires s.ready
   requires s.W()
   requires |LruModel.I(s.lru.Queue)| <= 0x1_0000_0000
-  //modifies s.Repr()
+  requires ImplModelCache.WriteAllocConditions(Ic(k), s.I())
   modifies s.lru.Repr
   modifies s.ephemeralIndirectionTable.Repr
+  modifies s.blockAllocator.Repr
   ensures s.ready
   ensures s.W()
+  ensures (s.I(), ref) == ImplModelCache.allocBookkeeping(Ic(k), old(s.I()), children)
   ensures forall o | o in s.lru.Repr :: o in old(s.lru.Repr) || fresh(o)
   ensures forall o | o in s.ephemeralIndirectionTable.Repr :: o in old(s.ephemeralIndirectionTable.Repr) || fresh(o)
-  ensures (s.I(), ref) == ImplModelCache.allocBookkeeping(Ic(k), old(s.I()), children)
+  ensures forall o | o in s.blockAllocator.Repr :: o in old(s.blockAllocator.Repr) || fresh(o)
   ensures |LruModel.I(s.lru.Queue)| <= |LruModel.I(old(s.lru.Queue))| + 1
-  //ensures s.cache.I() == old(s.cache.I())
   {
     ImplModelCache.reveal_allocBookkeeping();
     
